reification mostly working, starting on cancellation

misc/group_automation.v
@@ -1,10 +1,12 @@
 Require Import
   Coq.Classes.Morphisms
+  FunInd Recdef
   Coq.Lists.List
   MathClasses.interfaces.abstract_algebra
   MathClasses.interfaces.orders
   MathClasses.theory.groups
-  MathClasses.implementations.peano_naturals.
+  MathClasses.implementations.peano_naturals
+  Psatz.
 
 Import ListNotations.
 
@@ -13,26 +15,33 @@ Section GroupAutomation.
 Context `{Group A}.
 
 Inductive gexp : Type :=
-  | Atomic   : A -> gexp
+  | Atomic   : nat -> gexp
   | Identity : gexp
   | GroupOp  : gexp -> gexp -> gexp
   | Inverse  : gexp -> gexp
   .
 
-Fixpoint height a : nat := match a with
-  | Atomic _    => 0
-  | Identity    => 0
-  | GroupOp a b => 1 + height a + height b
-  | Inverse a   => 1 + height a
+Fixpoint gexp_denote (env : list A) (e : gexp) : A := match e with
+  | Atomic n => List.nth n env mon_unit
+  | Identity => mon_unit
+  | GroupOp a b => gexp_denote env a & gexp_denote env b
+  | Inverse a => - (gexp_denote env a)
   end.
 
-(*
-Lemma height_right : ∀ a b, height a < height (GroupOp a b).
-Proof. intros; simpl; repeat red.
-apply order_preserving. apply _.
-*)
+Fixpoint gexp_list_denote (env : list A) (e : list gexp) : A := match e with
+  | []    => mon_unit
+  | e::es => gexp_denote env e & gexp_list_denote env es
+  end.
 
-Program Fixpoint flatten (e : gexp) {measure (height e)} : list gexp :=
+Fixpoint gexp_height a : nat := match a with
+  | Atomic _    => 0
+  | Identity    => 0
+  | GroupOp a b => 1 + gexp_height a + gexp_height b
+  | Inverse a   => 1 + gexp_height a
+  end.
+
+(* flatten produces a list that only contains Atomics and Inverse Atomics *)
+Function flatten (e : gexp) {measure gexp_height} : list gexp :=
   match e with
   | GroupOp a b           => flatten a ++ flatten b
   | Inverse (GroupOp a b) => flatten (Inverse b) ++ flatten (Inverse a)
@@ -42,16 +51,105 @@ Program Fixpoint flatten (e : gexp) {measure (height e)} : list gexp :=
   | Identity              => []
   | Atomic a              => [Atomic a]
 end.
-Solve All Obligations with program_simpl; simpl; red; repeat match goal with
-  | [ |- (?x <= ?y)%nat ]         => setoid_replace ((x <= y)%nat) with (x ≤ y) by reflexivity
-  | [ |- context[(?x + ?y)%nat] ] => setoid_replace ((x + y)%nat) with (x + y) by reflexivity
-  | [ |- S _ ≤ S _ ]    => apply order_preserving; [apply _ | idtac]
-  | [ |- ?x ≤ ?x + ?y ] => setoid_replace x with (x + 0) at 1 by (symmetry; apply right_identity)
-                           ; apply order_preserving; [ apply _ | idtac ]
-  | [ |- ?x ≤ ?y + ?x ] => setoid_replace (y + x) with (x + y) by apply commutativity
-  | [ |- 0 ≤ ?x ]       => apply le_0_n
-  | [ |- ?x ≤ ?x ]      => constructor
-  | [ |- ?x ≤ S ?x ]    => constructor
+all: intros; simpl; lia.
+Defined.
+
+Lemma denote_append : ∀ env a b, gexp_list_denote env (a ++ b) = (gexp_list_denote env a) & (gexp_list_denote env b).
+Proof. induction a.
+  intros. simpl. rewrite left_identity. reflexivity.
+  intros. simpl. rewrite <- associativity. apply sg_op_proper. reflexivity. apply IHa. Qed.
+
+Theorem flatten_correct: ∀ (env : list A) (e : gexp),
+  gexp_denote env e = gexp_list_denote env (flatten e).
+Proof. intros env e; functional induction (flatten e); simpl.
+  rewrite denote_append. rewrite IHl. rewrite IHl0. reflexivity.
+  rewrite denote_append. rewrite <- IHl. rewrite <- IHl0. simpl. apply negate_sg_op_distr_flip.
+  apply negate_mon_unit.
+  rewrite IHl. apply involutive.
+  rewrite right_identity. reflexivity.
+  reflexivity.
+  rewrite right_identity. reflexivity.
+Qed.
+
+Function cancel (es : list gexp) {measure length} := 
+match es with Atomic n :: Inverse (Atomic m) :: es' => if decide (n = m) then cancel es' else Atomic n :: cancel (Inverse (Atomic m) :: es')
+  | Inverse (Atomic n) :: Atomic m :: es' => if decide (n = m) then cancel es' else Inverse (Atomic n) :: cancel (Atomic m :: es')
+  | x :: es' => x :: cancel es'
+  | [] => []
+end.
+all: simpl; intros; repeat constructor.
+Defined.
+
+Lemma cancel_correct: ∀ env es, gexp_list_denote env es = gexp_list_denote env (cancel es).
+Proof. intros env es. functional induction cancel es.
+  simpl. rewrite associativity. rewrite _x. rewrite right_inverse. rewrite left_identity. apply IHl.
+  simpl. rewrite <- IHl. simpl. reflexivity.
+  simpl. rewrite associativity. rewrite _x. rewrite left_inverse. rewrite left_identity. apply IHl.
+  simpl. rewrite IHl. reflexivity.
+  simpl. rewrite IHl. reflexivity.
+  reflexivity.
+Qed.
+
+Theorem group_reflect : ∀ env e1 e2,
+  gexp_list_denote env (flatten e1) = gexp_list_denote env (flatten e2)
+  -> gexp_denote env e1 = gexp_denote env e2.
+Proof. intros. rewrite flatten_correct. rewrite flatten_correct. assumption.
+Qed.
+
+Ltac inList x xs := match xs with
+  | []      => false
+  | x::_    => true
+  | _::?xs' => inList x xs'
+  end.
+
+Ltac addToList x xs :=
+  let b := inList x xs in
+  match b with
+    | true => xs
+    | false => constr:(x::xs)
+  end.
+
+Ltac lookup x xs := match xs with
+  | x::_    => O
+  | _::?xs' => let n := (lookup x xs') in
+               constr:(S n)
+  | _ => fail "no match for" x "in" xs
+  end.
+
+Ltac allVars xs e := match e with
+  | (?x = ?y) => let xs' := allVars xs x in
+                 allVars xs' y
+  | (?x & ?y) => let xs' := allVars xs x in
+                 allVars xs' y
+  | (- ?x)    => allVars xs x
+  | mon_unit  => xs
+  | _         => addToList e xs
 end.
 
+Ltac reifyTerm xs e :=
+let _ := match goal with | _ => idtac "reifyTerm" e end in
+match e with
+  | (?x = ?y) => let a := reifyTerm xs x in
+                 let b := reifyTerm xs y in
+                 constr:((a,b))
+  | (?x & ?y) => let a := reifyTerm xs x in
+                 let b := reifyTerm xs y in
+                 constr:(GroupOp a b)
+  | (- ?x)    => let a := reifyTerm xs x in
+                 constr:(Inverse a)
+  | mon_unit  => constr:(Identity)
+  | _         => let n := lookup e xs in
+                 constr:(Atomic n)
+  end.
 
+Ltac reify := match goal with
+  | [ |- ?ge1 = ?ge2 ] => let vars := allVars (nil : list A) ge1 in
+                          let vars := allVars vars ge2 in
+                          let e1   := reifyTerm vars ge1 in
+                          let e2   := reifyTerm vars ge2 in
+                          change (gexp_denote vars e1 = gexp_denote vars e2);
+                          apply group_reflect; simpl
+end.
+
+Lemma foo : ∀ x y z, x & -y & -(z & y) = x & -z.
+Proof. intros. reify. 
